simulations for stack operations

CoqOfRust/revm/simulations/arithmetic.v
@@ -376,20 +376,125 @@ End SharedMemory.
 *)
 
 Module Stack.
-  Record t : Set := {
-    data : list U256;
-  }.
+  Inductive t : Set :=
+  | data : list U256 -> t.
 
   Global Instance IsToTy : ToTy t := {
     Φ := Ty.path "revm_interpreter::interpreter::stack::Stack";
   }.
 
   Global Instance IsToValue : ToValue t := {
-    φ x :=
-      Value.StructRecord "revm_interpreter::interpreter::stack::Stack" [
-        ("data", φ x.(data))
-      ];
+    φ '(data x) := 
+      Value.StructRecord "revm_interpreter::interpreter::stack::Stack" [("data", φ x)]
   }.
+          
+  (*
+    /// Returns the length of the stack in words.
+    #[inline]
+    pub fn len(&self) -> usize {
+        self.data.len()
+    }
+  *)
+  Definition len '(data stack) : Z :=
+    Z.of_nat (List.length stack).
+
+  (*
+    /// Removes the topmost element from the stack and returns it, or `StackUnderflow` if it is
+    /// empty.
+    #[inline]
+    pub fn pop(&mut self) -> Result<U256, InstructionResult> {
+        self.data.pop().ok_or(InstructionResult::StackUnderflow)
+    }
+  *)
+  Definition pop :
+      MS? t string (U256 + InstructionResult.t) :=
+    letS? '(data stack) := readS? in
+    match stack with
+    | [] => returnS? (inr InstructionResult.StackUnderflow)
+    | x :: xs => 
+      letS? _ := writeS? (data xs) in
+      returnS? (inl x)
+    end.
+
+  (*
+    /// Removes the topmost element from the stack and returns it.
+    ///
+    /// # Safety
+    ///
+    /// The caller is responsible for checking the length of the stack.
+    #[inline]
+    pub unsafe fn pop_unsafe(&mut self) -> U256 {
+        self.data.pop().unwrap_unchecked()
+    }
+  *)
+  Definition pop_unsafe :
+      MS? t string U256 :=
+    letS? result := pop in
+    match result with
+    | inl x => returnS? x
+    | inr _ => panicS? "Stack underflow"
+    end.
+
+  (*
+      /// Peeks the top of the stack.
+      ///
+      /// # Safety
+      ///
+      /// The caller is responsible for checking the length of the stack.
+      #[inline]
+      pub unsafe fn top_unsafe(&mut self) -> &mut U256 {
+          let len = self.data.len();
+          self.data.get_unchecked_mut(len - 1)
+      }
+  *)
+  Definition top_unsafe :
+      MS? t string U256 :=
+    letS? '(data stack) := readS? in
+    match stack with
+    | [] => panicS? "Stack underflow"
+    | x :: _ => returnS? x
+    end.
+
+  (*
+      /// Pop the topmost value, returning the value and the new topmost value.
+      ///
+      /// # Safety
+      ///
+      /// The caller is responsible for checking the length of the stack.
+      #[inline]
+      pub unsafe fn pop_top_unsafe(&mut self) -> (U256, &mut U256) {
+          let pop = self.pop_unsafe();
+          let top = self.top_unsafe();
+          (pop, top)
+      }
+  *)
+  Definition pop_top_unsafe :
+      MS? t string (U256 * U256) :=
+    letS? pop := pop_unsafe in
+    letS? top := top_unsafe in
+    returnS? (pop, top).
+  
+  (*
+    /// Pops 2 values from the stack and returns them, in addition to the new topmost value.
+    ///
+    /// # Safety
+    ///
+    /// The caller is responsible for checking the length of the stack.
+    #[inline]
+    pub unsafe fn pop2_top_unsafe(&mut self) -> (U256, U256, &mut U256) {
+        let pop1 = self.pop_unsafe();
+        let pop2 = self.pop_unsafe();
+        let top = self.top_unsafe();
+
+        (pop1, pop2, top)
+    }
+  *)
+  Definition pop2_top_unsafe :
+      MS? t string (U256 * U256 * U256) :=
+    letS? pop1 := pop_unsafe in
+    letS? pop2 := pop_unsafe in
+    letS? top := top_unsafe in
+    returnS? (pop1, pop2, top).
 End Stack.
 
 (*
